

Derivation of Gradient Descent

Cost function in Linear Regression \rightarrow MSE (Mean squared error).

$$J(w, b) = \frac{1}{2m} \sum_{i=1}^m (f_{w,b}(x^{(i)}) - y^{(i)})^2$$

where $f_{w,b}(x) = wx + b$ $m \rightarrow$ no. of tuples.

Gradient Descent algorithm \rightarrow

$$w = w - \alpha \frac{\partial J(w, b)}{\partial w}$$

$$b = b - \alpha \frac{\partial J(w, b)}{\partial b}$$

(Repeat until convergence).

$$\frac{\partial}{\partial w} J(w, b) = \frac{\partial}{\partial w} \frac{1}{2m} \sum_{i=1}^m (f_{w,b}(x^{(i)}) - y^{(i)})^2$$

$$\Rightarrow \frac{\partial}{\partial w} \frac{1}{2m} \sum_{i=1}^m (wx^{(i)} + b - y^{(i)})^2$$

$$\Rightarrow \frac{1}{2m} \sum_{i=1}^m (wx^{(i)} + b - y^{(i)})^2 \cdot x \cdot x^{(i)}$$

$$\Rightarrow \frac{1}{m} \sum_{i=1}^m (wx^{(i)} + b - y^{(i)}) \cdot x^{(i)}$$

(By applying chain rule).

$$\frac{\partial}{\partial w} J(w, b) = \frac{1}{m} \sum_{i=1}^m (f_{w,b}(x^{(i)}) - y^{(i)}) \cdot x^{(i)}$$

$$\frac{\partial J(w, b)}{\partial b} = \frac{\partial}{\partial b} \frac{1}{2m} \sum_{i=1}^m \left(\cancel{f(w, b)} f_{w, b}(x^{(i)}) - y^{(i)} \right)^2$$

$$\Rightarrow \frac{\partial}{\partial b} \frac{1}{2m} \sum_{i=1}^m \left(w x^{(i)} + b - y^{(i)} \right)^2$$

$$\Rightarrow \frac{1}{2m} \sum_{i=1}^m \left(w x^{(i)} + b - y^{(i)} \right) \cdot 2$$

$$\Rightarrow \frac{1}{m} \sum_{i=1}^m \left(w x^{(i)} + b - y^{(i)} \right)$$

$$\frac{\partial J(w, b)}{\partial b} = \frac{1}{m} \sum_{i=1}^m \left(f_{w, b}(x^{(i)}) - y^{(i)} \right)$$

$$w = w - \alpha \sum_{i=1}^m \left(f_{w, b}(x^{(i)}) - y^{(i)} \right) x^{(i)}$$

$$b = b - \alpha \sum_{i=1}^m \left(f_{w, b}(x^{(i)}) - y^{(i)} \right)$$

Gradient descent for linear regression (MSE)